Remove TrySync interface

fstar/new/Crypto.fsti
@@ -8,6 +8,8 @@ open Lib.LoopCombinators
 open Lib.RandomSequence
 open Lib.Result
 
+#set-options "--z3rlimit 150"
+
 (** Definition of bytes *)
 (* val bytes : Type0 *)
 (* val length_of_bytes: bytes -> nat *)
@@ -15,44 +17,46 @@ open Lib.Result
 
 
 (** Definition of concrete bytes *)
-let bytes = Lib.Sequence.seq uint8
+let bytes_t = Seq.seq nat
+let pub_bytes_t = Seq.seq nat
+
 (* Empty bytes *)
 let empty_bytes = Seq.empty
 
 (* Conversion from integers to public bytes *)
-val nat_to_bytes: nat -> bytes
-val nat_to_n_bytes: nat -> nat -> bytes
-val nat_of_bytes: bytes -> result nat
+val nat_to_bytes: nat -> bytes_t
+val nat_to_n_bytes: nat -> nat -> bytes_t
+val nat_of_bytes: bytes_t -> result nat
 
 (* Concatenation and split for public bytes *)
-val concat: bytes -> bytes -> bytes
-val split: bytes -> result (bytes & bytes)
-val split_lemma1: a:bytes -> b:bytes ->
+val concat: bytes_t -> bytes_t -> bytes_t
+val split: bytes_t -> result (bytes_t & bytes_t)
+val split_lemma1: a:bytes_t -> b:bytes_t ->
     Lemma (ensures (split (concat a b) == Success (a,b)))
     [SMTPat (split (concat a b))]
-val split_lemma2: m:bytes ->
+val split_lemma2: m:bytes_t ->
     Lemma (match split m with
            | Success (a,b) -> m == concat a b
 	   | _ -> True)
     [SMTPat (split m)]
 
-val derive: bytes -> string -> bytes -> result bytes
-val derive_extract: bytes -> bytes -> result bytes
-val derive_expand_label: bytes -> string -> bytes -> nat -> result bytes
+val derive: bytes_t -> string -> bytes_t -> result bytes_t
+val derive_extract: bytes_t -> bytes_t -> result bytes_t
+val derive_expand_label: bytes_t -> string -> bytes_t -> nat -> result bytes_t
 
-val secret_to_public: bytes -> result pub_bytes
-val pke_enc: pub_bytes -> bytes -> result pub_bytes
-val pke_dec: bytes -> pub_bytes -> result bytes
+val secret_to_public: bytes_t -> result pub_bytes_t
+val pke_enc: pub_bytes_t -> bytes_t -> result pub_bytes_t
+val pke_dec: bytes_t -> pub_bytes_t -> result bytes_t
 
-val sign: bytes -> bytes -> result bytes
-val verify: bytes -> bytes -> bytes -> bool
+val sign: bytes_t -> bytes_t -> result bytes_t
+val verify: bytes_t -> bytes_t -> bytes_t -> bool
 
-val aead_enc: s:bytes -> b:bytes -> n:bytes -> ad:bytes -> result bytes
-val aead_dec: s:bytes -> enc:bytes -> n:bytes -> ad:bytes -> result bytes
+val aead_enc: s:bytes_t -> b:bytes_t -> n:bytes_t -> ad:bytes_t -> result bytes_t
+val aead_dec: s:bytes_t -> enc:bytes_t -> n:bytes_t -> ad:bytes_t -> result bytes_t
 
-val pad: bytes -> nat -> result bytes
-val unpad: bytes -> result bytes
+val pad: bytes_t -> nat -> result bytes_t
+val unpad: bytes_t -> result bytes_t
 
-val hash: bytes -> result bytes
-val mac: bytes -> bytes -> result bytes
-val mac_verify: bytes -> bytes -> bytes -> bool
+val hash: bytes_t -> result bytes_t
+val mac: bytes_t -> bytes_t -> result bytes_t
+val mac_verify: bytes_t -> bytes_t -> bytes_t -> bool
